adding properties 'sub_com' and 'branch_equiv'

SpecRelative.v
@@ -30,21 +30,21 @@ Set Default Goal Selector "!".
     speculative non-interference" from the paper "Hardware-Software Contracts
     for Secure Speculation" (IEEE SP 2021). *)
 
-Definition seq_obs_secure c st1 st2 ast1 ast2 :Prop :=
-  forall stt1 stt2 astt1 astt2 os1 os2,
+Definition seq_obs_secure c st1 st2 :Prop :=
+  forall ast1 ast2 stt1 stt2 astt1 astt2 os1 os2,
     <(st1, ast1)> =[ c ]=> <(stt1, astt1, os1)> ->
     <(st2, ast2)> =[ c ]=> <(stt2, astt2, os2)> ->
     os1 = os2.
 
-Definition spec_obs_secure c st1 st2 ast1 ast2 :Prop :=
-  forall ds stt1 stt2 astt1 astt2 bt1 bt2 os1 os2,
+Definition spec_obs_secure c st1 st2 :Prop :=
+  forall ds ast1 ast2 stt1 stt2 astt1 astt2 bt1 bt2 os1 os2,
     <(st1, ast1, false, ds)> =[ c ]=> <(stt1, astt1, bt1, os1)> ->
     <(st2, ast2, false, ds)> =[ c ]=> <(stt2, astt2, bt2, os2)> ->
     os1 = os2.
 
-Definition relative_secure (trans : com -> com) (c:com) (st1 st2:state) (ast1 ast2 :astate) : Prop :=
-  seq_obs_secure c st1 st2 ast1 ast2 ->
-  spec_obs_secure (trans c) st1 st2 ast1 ast2.
+Definition relative_secure (trans : com -> com) (c:com) (st1 st2:state) : Prop :=
+  seq_obs_secure c st1 st2  -> 
+  spec_obs_secure (trans c) st1 st2.  
 
 (** * Standard Speculative Load Hardening (SLH, not selective *)
 
@@ -78,23 +78,66 @@ Conjecture ideal_eval_no_spec_to_seq : forall P c s ast ds s' ast' os,
   <( s, ast )> =[ c ]=> <( s', ast', os )>.
 
 Theorem relative_secure_slh :
-  forall c st1 st2 ast1 ast2,
+  forall c st1 st2,
     (* some extra assumptions needed by slh_bcc *)
     unused "b" c ->
     st1 "b" = 0 ->
     st2 "b" = 0 ->
-    relative_secure slh c st1 st2 ast1 ast2.
+    relative_secure slh c st1 st2.
 Proof.
   unfold relative_secure, seq_obs_secure, spec_obs_secure.
-  intros c st1 st2 ast1 ast2 Hunused Hst1b Hst2b Hseq ds stt1 stt2 astt1 astt2 bt1 bt2 os1 os2 Hev1 Hev2.
+  intros c st1 st2 Hunused Hst1b Hst2b Hseq ds ast1 ast2 stt1 stt2 astt1 astt2 bt1 bt2 os1 os2 Hev1 Hev2.
   apply slh_bcc in Hev1; try assumption.
   apply slh_bcc in Hev2; try assumption.
   eapply same_final_b in Hev1 as SameB; try eassumption. subst.
   destruct bt1 eqn:Eqbt1.
-  - (* with speculation *) admit. (* ... the difficult case ... *)
+  - (* with speculation *)
+    destruct c as [| X e | c1 c2 | be ct cf | be cw | X a ie | a ie e ] eqn:Eqnc;
+    inversion Hev1; subst; clear Hev1; inversion Hev2; subst; clear Hev2;
+    simpl in *; eauto.
+    + (* Ideal_Seq *) admit.
+    + (* Ideal_If *) admit.
+    + (* Ideal If_F *) admit.
+    + (* Ideal_While *) admit.
   - (* without speculation *)
     pose proof (ideal_eval_no_spec _ _ _ _ _ _ _ _ Hev1) as NoSpec.
     eapply ideal_eval_no_spec_to_seq in Hev1; try assumption.
     eapply ideal_eval_no_spec_to_seq in Hev2; try assumption.
     eauto.
+Admitted.
+
+Fixpoint sub_com (c1 c2 :com) :Prop :=
+  match c2 with 
+  | <{{ c21; c22 }}> => c1 = c2 \/ sub_com c1 c21 \/ sub_com c1 c22
+  | <{{ if be2 then ct2 else cf2 end }}> =>
+        c1 = c2 \/ sub_com c1 ct2 \/ sub_com c1 cf2
+  | <{{ while be2 do cw2 end }}> => c1 = c2 \/ sub_com c1 cw2
+  | _ => c1 = c2
+  end.
+
+Lemma sub_com_refl : forall c, sub_com c c.
+Proof. destruct c; simpl; auto. Qed.
+
+Lemma sub_com_seq_obs_secure : forall c1 c2 st1 st2,
+  spec_obs_secure c2 st1 st2 ->
+  sub_com c1 c2 ->
+  spec_obs_secure c1 st1 st2.
+Proof.
+Admitted.
+
+Fixpoint branching_on_bexp (be :bexp) (c :com) :Prop :=
+  match c with
+  | <{{ c1; c2 }}> =>  branching_on_bexp be c1 \/ branching_on_bexp be c2
+  | <{{ if be' then ct else cf end }}> => 
+        be = be' \/ branching_on_bexp be ct \/ branching_on_bexp be cf
+  | <{{ while be' do cw end }}> => be = be' \/ branching_on_bexp be cw
+  | _  => False
+  end.
+
+Definition branch_equiv (c :com) (st1 st2 :state) :Prop :=
+  forall be, branching_on_bexp be c -> beval st1 be = beval st2 be.
+
+Lemma branch_equiv_seq_obs_secure : forall c st1 st2,
+  branch_equiv c st1 st2 ->
+  seq_obs_secure c st1 st2.
 Admitted.
